theories/monads.v
@@ -1,93 +1,10 @@
-From Coq Require Import Morphisms.
-From ExtLib.Structures Require Export Monads MonadLaws.
-From ITree Require Export Monad Basics.
+(* TODO define our own Monad class and remove the dependencies
+   on coq-extlib and coq-itree? *)
 
-(* TODO this file needs cleaning up *)
+From ExtLib.Structures Require Export Monads MonadLaws.
+From ITree Require Export Monad.
+
+(* Tactics. *)
 
 Ltac false :=
   elimtype False.
-
-Class MonadFlip (m : Type -> Type) := {
-  mflip: m bool
-}.
-
-Section MonadFixLaws.
-
-Context {m : Type -> Type}.
-
-(* The type class MonadFixLaws in coq-ext-lib does not work for us,
-   so we replace it with the following class. *)
-
-Class MonadFixLaws (MF : MonadFix m) := {
-  mleq :
-    forall {A}, m A -> m A -> Prop;
-  mleq_reflexive :
-    forall {A} (m : m A),
-    mleq m m;
-  mleq_transitive :
-    forall {A} (m1 m2 m3 : m A),
-    mleq m1 m2 -> mleq m2 m3 -> mleq m1 m3;
-  mfix_fixed_point :
-    forall {T A} (ff : (T -> m A) -> (T -> m A)),
-    (forall p1 p2,
-      (forall t, mleq (p1 t) (p2 t)) ->
-      (forall t, mleq (ff p1 t) (ff p2 t))) ->
-    mfix ff = ff (mfix ff)
-}.
-
-Class MonadFixCoinduction (MF : MonadFix m) (MFL : MonadFixLaws MF) := {
-  mfix_coinduction :
-    forall {T A} (ff : (T -> m A) -> (T -> m A)) (p : T -> m A),
-    (forall t, mleq (p t) (ff p t)) ->
-    (forall t, mleq (p t) (mfix ff t))
-}.
-
-End MonadFixLaws.
-
-Polymorphic Class MonadSkip (m : Type -> Type) : Type :=
-  skip : forall {A}, m A -> m A.
-
-Section MonadSkipLaws.
-
-Context {m : Type -> Type}.
-
-Context (M : Monad m).
-Context (MS : MonadSkip m).
-
-Class MonadSkipLaws := {
-  bind_skip :
-    forall A B (c : m A) (f : A -> m B),
-    bind (skip c) f = skip (bind c f)
-}.
-
-End MonadSkipLaws.
-
-(* ITree.Basics.CategoryTheory defines the type class [IterUnfold],
-   which is related to the statement below, but is unfortunately
-   stated in a more abstract way. *)
-
-Section MonadIterLaws.
-
-Context {m : Type -> Type}.
-
-Context (M : Monad m).
-Context (MI : MonadIter m).
-Context (MS : MonadSkip m).
-
-Class MonadIterLaws := {
-  unfold_iter :
-    forall {R I} (body : I -> m (I + R)) (i : I),
-    iter body i =
-      (* Evaluate [body] out the state [i]. *)
-      bind (body i) (fun (signal : I + R) =>
-        match signal with
-        | inl j =>
-            (* If the body yields a new state [j], continue. *)
-            skip (iter body j)
-        | inr r =>
-            (* If the body yields a result [r], return this result. *)
-            ret r
-        end)
-  }.
-
-End MonadIterLaws.
